Prove more permutation lemmas

JaEval.v
@@ -184,268 +184,7 @@ Proof.
 Admitted.
 
 (* ======================= Evaluation on extended heap ======================= *)
-Fixpoint LocsPermuted ls ls' pi :=
-  match (ls, ls') with
-  | ([], []) => True
-  | (l::ls, l'::ls') => PiMapsTo l l' pi /\ LocsPermuted ls ls' pi
-  | _ => False
-  end.
 
-Fixpoint ValsPermuted vs vs' pi :=
-  match (vs, vs') with
-  | ([], []) => True
-  | (JFVLoc v::vs, JFVLoc v'::vs') => PiMapsTo v v' pi /\ ValsPermuted vs vs' pi
-  | _ => False
-  end.
-
-Fixpoint ExprsPermuted e e' pi :=
-  match (e, e') with
-  | (JFNew mu cn vs, JFNew mu' cn' vs') =>
-      mu = mu' /\ cn = cn' /\
-      ValsPermuted vs vs' pi
-  | (JFLet cn x e1 e2, JFLet cn' x' e1' e2') =>
-      cn = cn' /\ x = x' /\
-      ExprsPermuted e1 e1' pi /\ ExprsPermuted e2 e2' pi
-  | (JFIf (JFVLoc v1) (JFVLoc v2) e1 e2, JFIf (JFVLoc v1') (JFVLoc v2') e1' e2') =>
-      ExprsPermuted e1 e1' pi /\ ExprsPermuted e2 e2' pi /\
-      PiMapsTo v1 v1' pi /\ PiMapsTo v2 v2' pi
-  | (JFInvoke (JFVLoc v1) m vs, JFInvoke (JFVLoc v1') m' vs') =>
-      PiMapsTo v1 v1' pi /\ ValsPermuted vs vs' pi /\ m = m'
-  | (JFAssign ((JFVLoc v1), _) (JFVLoc v2), JFAssign ((JFVLoc v1'), _) (JFVLoc v2')) =>
-      PiMapsTo v1 v1' pi /\ PiMapsTo v2 v2' pi
-  | (JFVal1 (JFVLoc v1), JFVal1 (JFVLoc v1')) =>
-      PiMapsTo v1 v1' pi
-  | (JFVal2 ((JFVLoc v1), _), JFVal2 ((JFVLoc v1'), _)) =>
-      PiMapsTo v1 v1' pi
-  | (JFThrow (JFVLoc v1), JFThrow (JFVLoc v1')) =>
-      PiMapsTo v1 v1' pi
-  | (JFTry e1 _ _ _ e2, JFTry e1' _ _ _ e2') =>
-      ExprsPermuted e1 e1' pi /\ ExprsPermuted e2 e2' pi
-  | _ => False
-  end.
-
-Definition CtxPermuted ctx ctx' pi :=
-  match (ctx, ctx') with
-  | (JFCtxLet cn x _ e2, JFCtxLet cn' x' _ e2') => cn = cn' /\ x = x' /\ ExprsPermuted e2 e2' pi
-  | (JFCtxTry _ _ cn x e2, JFCtxTry _ _ cn' x' e2') => cn = cn' /\ x = x' /\ ExprsPermuted e2 e2' pi
-  | _ => False
-  end.
-
-Fixpoint CtxsPermuted ctxs ctxs' pi :=
-  match (ctxs, ctxs') with
-  | ([], []) => True
-  | (ctx::ctxs, ctx'::ctxs') => CtxPermuted ctx ctx' pi /\ CtxsPermuted ctxs ctxs' pi
-  | _ => False
-  end.
-
-Definition FramesPermuted f f' pi :=
-  match (f, f') with
-  | (MkFrame ctxs e A, MkFrame ctxs' e' A') =>
-      ExprsPermuted e e' pi /\ CtxsPermuted ctxs ctxs' pi /\ A = A'
-  end.
-
-Fixpoint StacksPermuted st st' pi :=
-  match (st, st') with
-  | ([], []) => True
-  | (f::st, f'::st') => FramesPermuted f f' pi /\ StacksPermuted st st' pi
-  | _ => False
-  end.
-
-Definition PermutationSubset (pi pi' : HeapPermutation) :=
-  forall l1 l2, PiMapsTo l1 l2 pi -> PiMapsTo l1 l2 pi'.
-
-Lemma PermutationSubsetTrans : forall pi1 pi2 pi3,
-  PermutationSubset pi1 pi2 ->
-  PermutationSubset pi2 pi3 ->
-  PermutationSubset pi1 pi3.
-Proof.
-  intros pi1 pi2 pi3 pi1_pi2 pi2_pi3 x l pi1_x_l.
-  now apply pi2_pi3, pi1_pi2.
-Qed.
-
-Lemma PiMapsToEqIff : forall l1 l2 l1' l2' pi,
-  Bijection pi ->
-  PiMapsTo l1 l1' pi ->
-  PiMapsTo l2 l2' pi ->
-  (l1 = l2 <-> l1' = l2').
-Proof.
-  intros l1 l2 l1' l2' pi bijection pi_l1 pi_l2.
-  split.
-  + intros l_eq.
-    unfold PiMapsTo in *.
-    destruct l1, l2, l1', l2'; try easy.
-    injection l_eq as n_eq.
-    rewrite <-n_eq in pi_l2.
-    assert (n1_eq := MapsToEq (fst pi) n n1 n2 pi_l1 pi_l2).
-    now rewrite n1_eq.
-  + intros l_eq.
-    unfold PiMapsTo in *.
-    destruct l1, l2, l1', l2'; try easy.
-    apply bijection in pi_l1.
-    apply bijection in pi_l2.
-    injection l_eq as n1_eq.
-    rewrite <-n1_eq in pi_l2.
-    assert (n_eq := MapsToEq (snd pi) n1 n n0 pi_l1 pi_l2).
-    now rewrite n_eq.
-Qed.
-
-Lemma ExistsPermutedResult : forall res A stn_ext pi',
-  StacksPermuted [ [] [[JFVal1 (JFVLoc res) ]]_ A] stn_ext pi' ->
-  exists res', PiMapsTo res res' pi' /\
-       stn_ext = [ [] [[JFVal1 (JFVLoc res') ]]_ A].
-Proof.
-  intros res A stn_ext pi'.
-  intros pi_st.
-  unfold StacksPermuted in pi_st.
-  destruct stn_ext; try destruct pi_st.
-  destruct stn_ext; try destruct H0.
-  unfold FramesPermuted in H.
-  destruct f.
-  destruct H as (pi_val & pi_ctxs & A_eq).
-  simpl in pi_ctxs.
-  destruct Ctx; try destruct pi_ctxs.
-  unfold ExprsPermuted in pi_val.
-  destruct E; try destruct pi_val.
-  destruct v; try destruct pi_val.
-  exists l.
-  now rewrite A_eq.
-Qed.
-
-Lemma PermutationPreservesClassName : forall h0 h0' h0_perm h0_ext n n_perm C pi,
-  PiMapsTo (JFLoc n) (JFLoc n_perm) pi ->
-  HeapsPermuted h0 h0_perm pi ->
-  JFIDisjointUnion h0_perm h0' h0_ext ->
-  getClassName h0 n = Some C ->
-  getClassName h0_ext n_perm = Some C.
-Proof.
-  intros h0 h0' h0_perm h0_ext n n_perm C pi.
-  intros pi_n pi_h union class_name.
-  unfold getClassName in *.
-  assert (exists o, Heap.find n h0 = Some o).
-    destruct (Heap.find n h0); try discriminate class_name.
-    now exists o.
-  destruct H as (o & n_o_h).
-  rewrite n_o_h in class_name.
-  destruct pi_h as (_ & locs_fst & _ & objs).
-  unfold PiMapsTo in pi_n.
-  assert (n_in_h : Heap.In n h0).
-    apply HeapFacts.elements_in_iff.
-    exists o.
-    now apply HeapFacts.elements_mapsto_iff, HeapFacts.find_mapsto_iff.
-  destruct (locs_fst n n_in_h) as (n_perm' & n_nperm'_pi & n_perm'_in_h_perm).
-  rewrite <-(MapsToEq (fst pi) n n_perm n_perm') in *; trivial.
-  apply HeapFacts.elements_in_iff in n_perm'_in_h_perm.
-  destruct n_perm'_in_h_perm as (o' & n'_o'_h').
-  apply HeapFacts.elements_mapsto_iff in n'_o'_h'.
-
-  apply HeapFacts.find_mapsto_iff in n_o_h.
-  destruct o as (o & cn), o' as (o' & cn').
-  injection class_name as C_eq.
-  destruct (objs n n_perm o cn o' cn') as (cn_eq & _); trivial.
-
-  apply HeapFacts.find_mapsto_iff in n_o_h.
-  assert (subheap : JFISubheap h0_perm h0_ext). apply union.
-  assert (n'_o'_h_ext := subheap n_perm (o', cn') n'_o'_h').
-  apply HeapFacts.find_mapsto_iff in n'_o'_h_ext.
-  now rewrite n'_o'_h_ext, <-cn_eq, C_eq.
-Qed.
-
-Lemma ExistsPermutedExpr : forall e pi,
-  exists e', ExprsPermuted e e' pi.
-Proof.
-Admitted.
-
-Lemma PermutationPreservesSubstExpr : forall e e' pi f l l' e_body e_body',
-  ExprsPermuted e_body e_body' pi ->
-  ExprsPermuted e e' pi ->
-  PiMapsTo l l' pi ->
-  substExpr f l e_body = e ->
-  substExpr f l' e_body' = e'.
-Proof.
-Admitted.
-
-Lemma SubstPermutedExpr : forall f l l' e e' pi,
-  ExprsPermuted e e' pi ->
-  PiMapsTo l l' pi ->
-  ExprsPermuted (substExpr f l e) (substExpr f l' e') pi.
-Proof.
-Admitted.
-
-Lemma PermutationPreservesSubstList : forall fs vs vs',
-  (forall f, In f fs -> f <> JFThis) ->
-  length fs = length vs ->
-  length vs = length vs' -> forall e_body e_body' n n' e pi,
-  ValsPermuted vs vs' pi ->
-  ExprsPermuted e_body e_body' pi ->
-  PiMapsTo (JFLoc n) (JFLoc n') pi ->
-  substList fs vs  (substExpr JFThis (JFLoc n) e_body) = Some e ->
-  exists e',
-  ExprsPermuted e e' pi /\
-  substList fs vs' (substExpr JFThis (JFLoc n') e_body') = Some e'.
-Proof.
-  intros fs vs vs' fs_not_this fs_length_eq vs_length_eq.
-  set (_fs := fs).
-  replace fs with _fs in fs_not_this; try now unfold _fs.
-  set (_vs := vs).
-  set (_vs' := vs').
-  replace _fs  with (fst (split (combine fs (combine vs vs')))) in *.
-  replace _vs  with (fst (split (snd (split (combine fs (combine vs vs')))))).
-  replace _vs' with (snd (split (snd (split (combine fs (combine vs vs')))))).
-  clear fs_length_eq vs_length_eq _fs _vs _vs'.
-  induction (combine fs (combine vs vs')); clear fs vs vs'.
-  + intros e_body e_body' n n' e pi.
-    intros pi_vs pi_body pi_n subst.
-    simpl in *.
-         destruct (ExistsPermutedExpr e pi) as (e' & pi_e).
-    exists e'.
-    split; trivial.
-    unfold substList in *.
-    injection subst as subst.
-    apply PermutationPreservesSubstExpr
-      with (e' := e') (e_body' := e_body') (l' := (JFLoc n')) (pi := pi) in subst; trivial.
-    now rewrite subst.
-  + intros e_body e_body' n n' e pi.
-    intros pi_vs pi_body pi_n subst.
-    destruct a as (f & (v & v')).
-    simpl in *.
-    destruct (split l) as (fs & vs_vs').
-    unfold fst, snd in *.
-    simpl in *.
-    unfold fst, snd in *.
-    destruct (split vs_vs') as (vs & vs').
-    destruct v; try discriminate subst.
-    destruct v'; try destruct pi_vs.
-    assert (next_f_not_this : (forall f : JFRef, In f fs -> f <> JFThis)).
-      intros f0 f0_in_fs. apply (fs_not_this f0). now apply or_intror.
-    rewrite SubstExprComm in subst; [ | now apply fs_not_this, or_introl].
-    destruct (IHl next_f_not_this (substExpr f l0 e_body) (substExpr f l1 e_body') n n' e pi)
-      as (e' & pi_e & subst'); trivial.
-    now apply SubstPermutedExpr.
-    rewrite SubstExprComm in subst'; [ | now apply neq_symmetry, fs_not_this, or_introl].
-    now exists e'.
-  + rewrite combine_split; trivial.
-    ++ unfold snd.
-       rewrite combine_split; trivial.
-    ++ rewrite combine_length.
-       rewrite <-vs_length_eq, <-fs_length_eq.
-       now rewrite min_r.
-  + rewrite combine_split; trivial.
-    ++ unfold snd.
-       rewrite combine_split; trivial.
-    ++ rewrite combine_length.
-       rewrite <-vs_length_eq, <-fs_length_eq.
-       now rewrite min_r.
-  + rewrite combine_split; trivial.
-    rewrite combine_length.
-    rewrite <-vs_length_eq, <-fs_length_eq.
-    now rewrite min_r.
-Qed.
-
-Lemma PermutedValsLengthEq: forall vs vs' pi,
-  ValsPermuted vs vs' pi ->
-  length vs = length vs'.
-Proof.
-Admitted.
 
 Lemma ExistsPermutedBody : forall CC h0 h0' h0_ext h0_perm n n_perm m vs vs_perm ctxs ctxs_perm st st_perm h' st' pi,
   HeapsPermuted h0 h0_perm pi ->
@@ -498,7 +237,7 @@ Proof.
     rewrite map_length.
     admit. (* TODO params length *)
   assert (vs_length_eq : length vs = length vs_perm).
-    now apply PermutedValsLengthEq with (pi := pi).
+    now apply PermutedValsLength with (pi := pi).
   assert (pi_body : ExprsPermuted (body_of_md md) (body_of_md md) pi).
     admit. (* TODO body permuted -- no locs in it *)
   destruct (PermutationPreservesSubstList (map JFVar (params_of_md md)) vs vs_perm fs_not_this fs_length_eq vs_length_eq (body_of_md md) (body_of_md md) n n_perm Es pi)
@@ -528,73 +267,6 @@ Lemma AllocOnExtendedHeap : forall h0 h0_perm h0' h0_ext pi CC cn locs locs_perm
 Proof.
 Admitted.
 
-Lemma EqualLengthInduction : forall {A} p (q : A -> A -> Prop),
-  p [] [] ->
-  (forall (x x' : A) xs xs', q x x' -> p xs xs' -> p (x::xs) (x'::xs')) ->
-  forall xs xs',
-    length xs = length xs' ->
-    p xs xs'.
-Proof.
-Admitted.
-
-Lemma ExtendCtxPermutation : forall ctx ctx_perm pi pi',
-  CtxPermuted ctx ctx_perm pi ->
-  PermutationSubset pi pi' ->
-  CtxPermuted ctx ctx_perm pi'.
-Proof.
-Admitted.
-
-Lemma PermutedCtxsLength : forall ctxs ctxs_perm pi,
-  CtxsPermuted ctxs ctxs_perm pi ->
-  length ctxs = length ctxs_perm.
-Proof.
-  intros ctxs.
-  induction ctxs;
-    intros ctxs_perm pi pi_ctxs;
-    destruct ctxs_perm; try now destruct pi_ctxs.
-  simpl in *.
-  now rewrite IHctxs with (ctxs_perm := ctxs_perm) (pi := pi).
-Qed.
-
-Ltac induction2 l1 l2 length_eq head1 head2 tail1 tail2 :=
-  set (_l1 := l1);
-  set (_l2 := l2);
-  (replace l1 with _l1 in *; try now unfold _l1);
-  (replace l2 with _l2 in *; try now unfold _l2);
-  (replace _l1 with l1 in length_eq; try now unfold _l1);
-  (replace _l2 with l2 in length_eq; try now unfold _l2);
-  (replace _l1 with (fst (split (combine l1 l2))) in *; try now rewrite combine_split);
-  (replace _l2 with (snd (split (combine l1 l2))) in *; try now rewrite combine_split);
-  clear _l1 _l2;
-  induction (combine l1 l2) as [ | _a _l];
-    [unfold split in *
-    | simpl in *; destruct _a as (head1 & head2), (split _l) as (tail1 & tail2)
-    ];
-  unfold fst, snd in *.
-
-Lemma ExtendCtxsPermutation : forall ctxs ctxs_perm pi pi',
-  CtxsPermuted ctxs ctxs_perm pi ->
-  PermutationSubset pi pi' ->
-  CtxsPermuted ctxs ctxs_perm pi'.
-Proof.
-  intros ctxs ctxs_perm pi pi' pi_ctx pi_subset.
-  assert (length_eq : length ctxs = length ctxs_perm).
-    now apply PermutedCtxsLength with (pi := pi).
-  induction2 ctxs ctxs_perm length_eq ctx ctx_perm ctxs' ctxs'_perm; try easy.
-  simpl in *.
-  destruct pi_ctx as (pi_ctx & pi_ctxs).
-  split.
-  now apply ExtendCtxPermutation with (pi := pi).
-  now apply IH_l.
-Qed.
-
-Lemma ExtendStacksPermutation : forall st st_perm pi pi',
-  StacksPermuted st st_perm pi ->
-  PermutationSubset pi pi' ->
-  StacksPermuted st st_perm pi'.
-Proof.
-Admitted.
-
 Lemma LocOfValsPermutation : forall vs locs vs_perm pi,
   list_map_opt loc_of_val vs = Some locs ->
   ValsPermuted vs vs_perm pi ->
@@ -602,7 +274,33 @@ Lemma LocOfValsPermutation : forall vs locs vs_perm pi,
     list_map_opt loc_of_val vs_perm = Some locs' /\
     LocsPermuted locs locs' pi.
 Proof.
-Admitted.
+  intros vs.
+  induction vs; intros locs vs_perm pi locs_of_vs pi_vs.
+  + exists [].
+    simpl in *.
+    destruct vs_perm; try destruct pi_vs.
+    injection locs_of_vs as locs_eq.
+    now rewrite <- locs_eq.
+  + simpl in *.
+    destruct a, vs_perm; try destruct j; try destruct pi_vs.
+    simpl in locs_of_vs.
+    destruct locs as [ | loc locs].
+      destruct (list_map_opt loc_of_val vs); try discriminate locs_of_vs.
+    assert (locs_of_vs' : list_map_opt loc_of_val vs = Some locs).
+      destruct (list_map_opt loc_of_val vs); try discriminate locs_of_vs.
+      injection locs_of_vs.
+      intros locs_eq _.
+      now rewrite locs_eq.
+    assert (l_eq : l = loc).
+      destruct (list_map_opt loc_of_val vs); try discriminate locs_of_vs.
+      now injection locs_of_vs.
+    rewrite l_eq in *.
+    destruct (IHvs locs vs_perm pi) as (locs' & locs'_of_vs_perm & pi_locs) ; try easy.
+    exists (l0::locs').
+    split; try easy.
+    simpl.
+    now rewrite locs'_of_vs_perm.
+Qed.
 
 Lemma ReductionPreservesHeapPermutation : forall h0 h0_perm h0' h0_ext st h' st' st_perm pi CC,
   PiMapsTo (JFLoc NPE_object_loc) (JFLoc NPE_object_loc) pi ->
